theories/LambdaCube/infer.v
@@ -1,0 +1,419 @@
+From Coq Require Import Utf8.
+From Coq Require Import Arith Lia.
+From FormArith Require Import Base.
+From FormArith.LambdaCube Require Import Term Operational Typing SN whnf normalize.
+
+Inductive strong_ctx_wf (Sc: pi_scheme) : forall {n}, typing_ctx n -> Type :=
+| strong_empty_wf : strong_ctx_wf Sc \
+| strong_cons_wf {n} {Γ: typing_ctx n} {A: term n} s :
+  strong_ctx_wf Sc Γ -> Γ ⊢(Sc) A : Srt s -> strong_ctx_wf Sc (Γ; A)
+.
+
+Lemma strong_to_weak_ctx_wf Sc {n} (Γ: typing_ctx n) : strong_ctx_wf Sc Γ -> Γ ⊢(Sc).
+Proof.
+  induction 1; econstructor; eassumption.
+Qed.
+
+Fixpoint kth_srt_ctx {Sc} {n} {Γ: typing_ctx n} (H: strong_ctx_wf Sc Γ) (k: nat) {struct H}
+  : k < n -> sort :=
+  match H with
+  | strong_empty_wf _ => fun H => match Nat.nlt_0_r k H with end
+  | @strong_cons_wf _ n _ _ s H _ =>
+      fun _ =>
+        match lt_dec k n with
+        | left l => kth_srt_ctx H k l
+        | right _ => s
+        end
+  end.
+
+Lemma kth_typ_index {Sc} {n} {Γ: typing_ctx n} (H: strong_ctx_wf Sc Γ) k (l : k < n) :
+  Γ ⊢(Sc) kth_index_ctx Γ k l : Srt (kth_srt_ctx H k l).
+Proof.
+  induction H; simpl. { destruct (Nat.nlt_0_r _ _). } destruct (lt_dec _ _).
+  - change (@Srt (S ?n) ?s) with (ren weaken (@Srt n s)). eapply weakening; eauto.
+  - change (@Srt (S ?n) ?s) with (ren weaken (@Srt n s)). eapply weakening; eassumption.
+Qed.
+
+Lemma SN_srt {n} s : SN (@Srt n s).
+Proof.
+  constructor. intros. exfalso. eapply no_srt_step. eassumption.
+Qed.
+
+Inductive infer_ret Sc {n} Γ (t: term n) : Type :=
+| Untyped
+| Kind (typt: Γ ⊢(Sc) t : Srt Box)
+| Sorted T s (typt: Γ ⊢(Sc) t : T) (typT: Γ ⊢(Sc) T : Srt s).
+
+Arguments Kind {_ _ _ _}.
+Arguments Sorted {_ _ _ _}.
+
+(* Sorted means we have a term that is neither a type nor a kind, along with its sort *)
+
+Fixpoint infer_aux Sc {n} {Γ} (H: strong_ctx_wf Sc Γ) (t: term n) {struct t}
+  : infer_ret Sc Γ t :=
+  match t with
+  | Srt Star => Kind (typ_star _ (strong_to_weak_ctx_wf _ _ H))
+  | Srt Box => Untyped _ _ _
+  | Var k =>
+      (*match kth_index_ctx Γ (proj1_sig k) (proj2_sig k)
+            as T return
+            Γ ⊢(Sc) Var k : T ->
+                            Γ ⊢(Sc) T : Srt (kth_srt_ctx H (proj1_sig k) (proj2_sig k)) -> _
+      with
+      | Srt Star => fun H _ => _
+      | T => fun typV typT => Sorted T _ typV typT
+      end*) Sorted _ _ (typ_var _ (strong_to_weak_ctx_wf _ _ H)) (kth_typ_index H _ _)
+  | Pi A B =>
+      match infer_aux Sc H A with
+      | Kind typA =>
+          match infer_aux Sc (strong_cons_wf _ _ H typA) B with
+          | Kind typB =>
+              (if Sc Box Box as b return Sc Box Box = b -> _
+               then fun e => Kind (typ_pi _ e typA typB)
+               else fun _ => Untyped _ _ _) eq_refl
+          | Sorted T s' typB typT =>
+              let H' := ex_intro _ _ (ex_intro _ _ (ex_intro _ _ typT)) in
+              match whnormalize_typed T H' as T' return Γ; A ⊢(Sc) B : T' -> _
+              with
+              | Srt Star =>
+                  fun typB =>
+                    (if Sc Box Star as b return Sc Box Star = b -> _
+                     then fun e =>
+                            Sorted _ _ (typ_pi _ e typA typB)
+                               (typ_star _ (strong_to_weak_ctx_wf _ _ H))
+                     else fun _ => Untyped _ _ _) eq_refl
+              | _ => fun _ => Untyped _ _ _
+              end (
+                  let H' : T ≻* whnormalize_typed T H' := whnormalize_typed_step_star _ _ in
+                  typ_conv _ typB (Requiv_clot_star H') (subject_reduction _ _ _ _ _ typT H')
+                )
+          | _ => Untyped _ _ _
+          end
+      | Sorted T s typA typT =>
+          let H' := ex_intro _ _ (ex_intro _ _ (ex_intro _ _ typT)) in
+          match whnormalize_typed T H' as T' return Γ ⊢(Sc) A : T' -> _
+          with
+          | Srt Star =>
+              fun typA =>
+                match infer_aux Sc (strong_cons_wf _ _ H typA) B with
+                | Kind typB =>
+                    (if Sc Star Box as b return Sc Star Box = b -> _
+                     then fun e => Kind (typ_pi _ e typA typB)
+                     else fun _ => Untyped _ _ _) eq_refl
+                | Sorted T s' typB typT =>
+                    let H' := ex_intro _ _ (ex_intro _ _ (ex_intro _ _ typT)) in
+                    match whnormalize_typed T H' as T' return Γ; A ⊢(Sc) B : T' -> _
+                    with
+                    | Srt Star =>
+                        fun typB =>
+                          (if Sc Star Star as b return Sc Star Star = b -> _
+                           then fun e =>
+                                  Sorted _ _ (typ_pi _ e typA typB)
+                                    (typ_star _ (strong_to_weak_ctx_wf _ _ H))
+                           else fun _ => Untyped _ _ _) eq_refl
+                    | _ => fun _ => Untyped _ _ _
+                    end (
+                        let H' : T ≻* whnormalize_typed T H' := whnormalize_typed_step_star _ _
+                        in typ_conv _ typB (Requiv_clot_star H')
+                             (subject_reduction _ _ _ _ _ typT H')
+                      )
+                | _ => Untyped _ _ _
+                end
+          | _ => fun _ => Untyped _ _ _
+          end (
+              let H' : T ≻* whnormalize_typed T H' := whnormalize_typed_step_star _ _ in
+              typ_conv _ typA (Requiv_clot_star H') (subject_reduction _ _ _ _ _ typT H')
+            )
+      | _ => Untyped _ _ _
+      end
+  | Abs A t =>
+      match infer_aux Sc H A with
+      | Kind typA =>
+          match infer_aux Sc (strong_cons_wf _ _ H typA) t with
+          | Kind typt => Untyped _ _ _
+          | Sorted B s' typt typB => 
+              (if Sc Box s' as b return Sc Box s' = b -> _
+               then fun e =>
+                      Sorted _ _
+                        (typ_abs _ e typA typB typt)
+                        (typ_pi _ e typA typB)
+               else fun _ => Untyped _ _ _) eq_refl
+          | _ => Untyped _ _ _
+          end
+      | Sorted T s typA typT =>
+          let H' := ex_intro _ _ (ex_intro _ _ (ex_intro _ _ typT)) in
+          match whnormalize_typed T H' as T' return Γ ⊢(Sc) A : T' -> _
+          with
+          | Srt Star =>
+              fun typA =>
+                match infer_aux Sc (strong_cons_wf _ _ H typA) t with
+                | Kind typt => Untyped _ _ _
+                | Sorted B s' typt typB => 
+                    (if Sc Star s' as b return Sc Star s' = b -> _
+                     then fun e =>
+                            Sorted _ _
+                              (typ_abs _ e typA typB typt)
+                              (typ_pi _ e typA typB)
+                     else fun _ => Untyped _ _ _) eq_refl
+                | _ => Untyped _ _ _
+                end
+          | _ => fun _ => Untyped _ _ _
+          end (
+              let H' : T ≻* whnormalize_typed T H' := whnormalize_typed_step_star _ _ in
+              typ_conv _ typA (Requiv_clot_star H') (subject_reduction _ _ _ _ _ typT H')
+            )
+      | _ => Untyped _ _ _
+      end
+  | App t u =>
+      match infer_aux Sc H t with
+      | Sorted T s' typt typT =>
+          let H' := ex_intro _ _ (ex_intro _ _ (ex_intro _ _ typT)) in
+          match whnormalize_typed T H' as T' return Γ ⊢(Sc) t : T' -> Γ ⊢(Sc) T' : Srt s' -> _
+          with
+          | Pi A B =>
+              fun typt typPi =>
+                (fun  H' : exists s, Γ ⊢(Sc) A : Srt s /\ Γ ; A ⊢(Sc) B: Srt s' =>
+                   match infer_aux Sc H u with
+                   | Sorted U s typu typU =>
+                       match convertible_typed (ex_intro _ _ typU)
+                               (let (s, H') := H' in
+                                let (typA, _) := H' in
+                                ex_intro _ _ typA)
+                       with
+                       | left Hconv =>
+                           Sorted _ _
+                             (typ_app _ typt
+                                (let (_, H') := H' in
+                                 let (typA, _) := H' in
+                                 typ_conv _ typu Hconv typA
+                             ))
+                             (let (_, H') := H' in
+                              let (typA, typB) := H' in
+                              bind_first_typ (typ_conv _ typu Hconv typA) typB :
+                                (Γ ⊢(Sc) _ : bind (bind_first u) (Srt s'))
+                             )
+                       | right _ => Untyped _ _ _
+                       end
+                   (* -2 Goal *)
+                   | Kind typu =>
+                       Untyped _ _ _
+                   | _ => Untyped _ _ _
+                   end
+                )
+                  (
+                    let (s, H') := typ_pi_inv _ _ _ _ _ typPi in
+                    let (s__c, H') := H' in
+                    let (srt_eq, H') := H' in
+                    let (typA, H') := H' in
+                    let (typB, _) := H' in
+                    ex_intro _ s (
+                        conj typA
+                          (
+                            let e := srt_equiv_srt srt_eq in
+                            match eq_sym e with
+                            | eq_refl => typB
+                            end
+                          )
+                      )
+                  )
+          | _ => fun _ _ => Untyped _ _ _
+          end
+            (typ_conv _ typt (Requiv_clot_star (whnormalize_typed_step_star _ _))
+               (whnormalize_typed_preserves _ _ _ _ _ typT)
+            )
+            (whnormalize_typed_preserves _ _ _ _ _ typT)
+      | _ => Untyped _ _ _
+      end
+  end.
+
+Lemma typed_infer_aux_not_untyped Sc {n} Γ (H: strong_ctx_wf Sc Γ) (t T: term n) :
+  Γ ⊢(Sc) t : T -> match infer_aux Sc H t with Untyped _ _ _ => False | _ => True end.
+Proof.
+  induction 1; simpl; auto.
+  - specialize (IHtyping1 H). destruct (infer_aux _ _ A) as [| typA |]; try tauto.
+    + assert (s = Box).
+      { eapply srt_equiv_srt. eapply unique_typing; eassumption. } subst.
+      clear H0_. rename H0 into pi_check.
+      specialize (IHtyping2 (strong_cons_wf _ _ H typA)).
+      destruct (infer_aux _ _ _); try tauto.
+      * generalize (@eq_refl _ (Sc Box Box)). generalize (Sc Box Box) at 2 3.
+        destruct b; try tauto. intro. unfold pi_scheme_check in *.
+        assert (s' = Box).
+        { eapply srt_equiv_srt. eapply unique_typing; eassumption. }
+        subst. congruence.
+      * assert (T ≻* Srt s').
+        { eapply srt_equiv. eapply unique_typing; try eassumption. }
+        match goal with |- context[match _ with _ => _ end ?x] => generalize x end.
+        set (whnormalize_typed _ _).
+        assert (t ≻* Srt s').
+        { eapply confluence_step in H0 as [v [norm_red srt_red]]; swap 1 2.
+          { apply whnormalize_typed_step_star. } apply srt_star in srt_red. subst.
+          exact norm_red. }
+        assert (t ≅ Srt s').
+        { apply Requiv_clot_star. assumption. }
+        assert (t = Srt s').
+        { pose proof (whnft := whnormalize_typed_whnf _ _ : whnf t).
+          epose proof (whnf_is_sort_type_or_never_will_be whnft).
+          destruct t; try firstorder. f_equal. eapply srt_equiv_srt. eassumption. }
+        rewrite H3.
+        assert (typs' : Γ; A ⊢(Sc) Srt s' : Srt s).
+        { eapply subject_reduction; try eassumption. }
+        assert (s' = Star).
+        { destruct s'; auto. exfalso. revert typs'. clear. generalize (@Srt (S n) s) as T. intro.
+          remember (Srt Box). induction 1 in Heqt |- *; try discriminate; tauto. }
+        subst. intro. generalize (@eq_refl _ (Sc Box Star)).
+        generalize (Sc Box Star) at 2 3. destruct b; auto. congruence.
+    + assert (T ≻* Srt s).
+        { eapply srt_equiv. eapply unique_typing; try eassumption. }
+        match goal with |- context[match _ with _ => _ end ?x] => generalize x end.
+        set (whnormalize_typed _ _).
+        assert (t ≻* Srt s).
+        { eapply confluence_step in H1 as [v [norm_red srt_red]]; swap 1 2.
+          { apply whnormalize_typed_step_star. } apply srt_star in srt_red. subst.
+          exact norm_red. }
+        assert (t ≅ Srt s).
+        { apply Requiv_clot_star. assumption. }
+        assert (t = Srt s).
+        { pose proof (whnft := whnormalize_typed_whnf _ _ : whnf t).
+          epose proof (whnf_is_sort_type_or_never_will_be whnft).
+          destruct t; try firstorder. f_equal. eapply srt_equiv_srt. eassumption. }
+        rewrite H4. clear dependent t.
+        assert (typs : Γ ⊢(Sc) Srt s : Srt s0) by (eauto using subject_reduction).
+        assert (s = Star).
+        { destruct s; auto. exfalso. revert typs. clear. generalize (@Srt (S n) s0) as T. intro.
+          remember (Srt Box). clear T. induction 1 in Heqt |- *; try discriminate; tauto. }
+        subst. intro typA. clear dependent T.
+        specialize (IHtyping2 (strong_cons_wf _ _ H typA)). destruct (infer_aux _ _ _); try tauto.
+      * generalize (@eq_refl _ (Sc Star Box)). generalize (Sc Star Box) at 2 3.
+        destruct b; try tauto. intro. unfold pi_scheme_check in *.
+        assert (s' = Box).
+        { eapply srt_equiv_srt. eapply unique_typing; eassumption. }
+        subst. congruence.
+      * assert (T ≻* Srt s').
+        { eapply srt_equiv. eapply unique_typing; try eassumption. }
+        match goal with |- context[match _ with _ => _ end ?x] => generalize x end.
+        set (whnormalize_typed _ _).
+        assert (t ≻* Srt s').
+        { eapply confluence_step in H1 as [v [norm_red srt_red]]; swap 1 2.
+          { apply whnormalize_typed_step_star. } apply srt_star in srt_red. subst.
+          exact norm_red. }
+        assert (t ≅ Srt s').
+        { apply Requiv_clot_star. assumption. }
+        assert (t = Srt s').
+        { pose proof (whnft := whnormalize_typed_whnf _ _ : whnf t).
+          epose proof (whnf_is_sort_type_or_never_will_be whnft).
+          destruct t; try firstorder. f_equal. eapply srt_equiv_srt. eassumption. }
+        rewrite H4.
+        assert (typs' : Γ; A ⊢(Sc) Srt s' : Srt s).
+        { eapply subject_reduction; try eassumption. }
+        assert (s' = Star).
+        { destruct s'; auto. exfalso. revert typs'. clear. generalize (@Srt (S n) s) as T. intro.
+          remember (Srt Box). induction 1 in Heqt |- *; try discriminate; tauto. }
+        subst. intro. generalize (@eq_refl _ (Sc Star Star)).
+        generalize (Sc Star Star) at 2 3. destruct b; auto. congruence.
+  - specialize (IHtyping1 H). destruct (infer_aux _ _ A); try tauto.
+    + specialize (IHtyping3 (strong_cons_wf _ Box H typt)).
+      destruct (infer_aux _ _ _); try tauto.
+      * cut (Γ; A ⊢(Sc) Srt Box : Srt s').
+        { clear. remember (Srt Box). induction 1 in Heqt |- *; try discriminate; tauto. }
+        eapply subject_reduction; try eassumption. eapply srt_equiv.
+        eapply unique_typing; try eassumption.
+      * generalize (@eq_refl _ (Sc Box s0)). generalize (Sc Box s0) at 2 3.
+        destruct b; auto.
+        assert (s = Box). {eapply srt_equiv_srt. eapply unique_typing; eassumption. }
+        subst. enough (s' = s0) by congruence.
+        assert (T ≅ B) by eauto using unique_typing.
+        apply (@srt_equiv_srt (S n)). revert H0_0 typT H1.
+        generalize (Γ; A) (@Srt (S n) s') (@Srt (S n) s0). clear.
+        rename B into t, T into u. intros Γ X Y typB typT Hcong.
+        eapply equiv_both_star in Hcong as [v [redu redt]].
+        eapply unique_typing; eapply subject_reduction; eauto.
+    + assert (T ≻* Srt s).
+      { eapply srt_equiv. eapply unique_typing; try eassumption. }
+      match goal with |- context[match _ with _ => _ end ?x] => generalize x end.
+      set (whnormalize_typed _ _) as u.
+      assert (u ≻* Srt s).
+      { eapply confluence_step in H1 as [v [norm_red srt_red]]; swap 1 2.
+        { apply whnormalize_typed_step_star. } apply srt_star in srt_red. subst.
+        exact norm_red. }
+      assert (u ≅ Srt s).
+      { apply Requiv_clot_star. assumption. }
+      assert (u = Srt s).
+      { pose proof (whnfu := whnormalize_typed_whnf _ _ : whnf u).
+        epose proof (whnf_is_sort_type_or_never_will_be whnfu).
+        destruct u; try firstorder. f_equal. eapply srt_equiv_srt. eassumption. }
+      rewrite H4. clear dependent u.
+      assert (typs : Γ ⊢(Sc) Srt s : Srt s0) by (eauto using subject_reduction).
+      assert (s = Star).
+      { destruct s; auto. exfalso. revert typs. clear. generalize (@Srt (S n) s0) as T. intro.
+        remember (Srt Box). clear T. induction 1 in Heqt |- *; try discriminate; tauto. }
+      subst. intro typA. clear dependent T.
+      specialize (IHtyping3 (strong_cons_wf _ _ H typA)). destruct (infer_aux _ _ _); try tauto.
+      * cut (Γ; A ⊢(Sc) Srt Box : Srt s').
+        { clear. remember (Srt Box). induction 1 in Heqt |- *; try discriminate; tauto. }
+        eapply subject_reduction; try eassumption. eapply srt_equiv.
+        eapply unique_typing; try eassumption.
+      * generalize (@eq_refl _ (Sc Star s)). generalize (Sc Star s) at 2 3.
+        destruct b; auto.
+        enough (s = s') by congruence.
+        assert (T ≅ B) by eauto using unique_typing.
+        apply (@srt_equiv_srt (S n)). revert H0_0 typT H1.
+        generalize (Γ; A) (@Srt (S n) s') (@Srt (S n) s0). clear.
+        rename B into t, T into u. intros Γ X Y typB typT Hcong.
+        eapply equiv_both_star in Hcong as [v [redu redt]].
+        eapply unique_typing; eapply subject_reduction; eauto.
+  - specialize (IHtyping1 H). destruct (infer_aux _ _ t); try tauto.
+    { assert (e: Srt Box ≅ Pi A B) by eauto using unique_typing.
+      eapply srt_equiv, pi_star in e. firstorder discriminate. }
+      match goal with |- context[match _ with _ => _ end ?x ?y] => generalize x y end.
+    set (whnormalize_typed _ _) as T'.
+    pose proof (whnft := whnormalize_typed_whnf _ _ : whnf T').
+    epose proof (whnf_is_pi_type_or_never_will_be whnft). intros typt' typT'.
+    assert (T' ≅ Pi A B) by eauto using unique_typing.
+    match goal with |- context[match _ with _ => _ end ?x typT'] => generalize x end.
+    destruct T'; try solve [firstorder]. intro typt''.
+    specialize (IHtyping2 H). destruct (infer_aux _ _ _); try tauto.
+    { assert (Hcong : A ≅ Srt Box) by eauto using unique_typing. revert H0_ Hcong. clear.
+      intros Htyp Hcong. apply srt_typing in Htyp as [|[s Htyp]]; try discriminate.
+      apply typ_pi_inv in Htyp as [s' [_ [_ [typA _]]]]. apply Requiv_sym, srt_equiv in Hcong.
+      assert (c : Γ ⊢(Sc) Srt Box: Srt s') by eauto using subject_reduction.
+      revert c. clear. remember (Srt Box). induction 1; try discriminate; tauto. }
+    destruct (convertible_typed _ _); auto.
+    apply n0. assert (Hcong : T0 ≅ A) by eauto using unique_typing.
+    apply (Requiv_trans Hcong). revert H1. clear. intro H. apply pi_equiv_pi in H.
+    intuition auto using Requiv_sym.
+  - apply IHtyping1.
+Qed.
+
+Definition infer Sc {n} {Γ} (H: strong_ctx_wf Sc Γ) (t: term n) : option (term n) :=
+  match infer_aux Sc H t with
+  | Untyped _ _ _ => None
+  | Kind _ => Some (Srt Box)
+  | Sorted T _ _ _ => Some T
+  end.
+
+Lemma infer_some Sc {n} {Γ} (H: strong_ctx_wf Sc Γ) (t: term n) T :
+  infer Sc H t = Some T -> Γ ⊢(Sc) t : T.
+Proof.
+  unfold infer.
+  destruct (infer_aux _ _ _); try discriminate; inversion 1; subst; auto.
+Qed.
+
+Lemma infer_none Sc {n} {Γ} (H: strong_ctx_wf Sc Γ) (t: term n) :
+  infer Sc H t = None -> forall T, ¬ (Γ ⊢(Sc) t : T).
+Proof.
+  unfold infer.
+  destruct (infer_aux _ _) eqn: e; try discriminate. intros _ T typt.
+  eapply typed_infer_aux_not_untyped in typt. rewrite e in typt. assumption.
+Qed.
+
+Definition infer_dec Sc {n} {Γ} (H: strong_ctx_wf Sc Γ) (t: term n) :
+  { T | Γ ⊢(Sc) t : T } + {forall T, ¬ (Γ ⊢(Sc) t : T)} :=
+  match infer Sc H t as o return infer Sc H t = o -> _ with
+     | None => fun e => inright (infer_none _ _ _ e)
+     | Some T => fun e => inleft (exist _ T (infer_some _ _ _ _ e))
+  end eq_refl.
+
+Definition infer_dec_closed Sc (t: term 0) :
+  { T | \ ⊢(Sc) t : T } + {forall T, ¬ (\ ⊢(Sc) t : T)} :=
+  infer_dec Sc (strong_empty_wf Sc) t.
